Add eq_reasoning to the current code
Update Hoare to put ...E lemmas rather than a tactic

Add to_hoare request API

Refactor hoarefacts proofs.

Messy tactic removing, this still needs a huge clean on airlock

Hoare after rebase

Update HoareFacts post rebase

Update airlock post rebase

First try to simplify

cleaning

minor

fix

broken

upd

small clean

Update the hoare helper lemmas

update with reynald

add warnings and deprecations

Update Interface to teffects.

rework imports locally

remove unused imports

Move Impure to FReer

small naming modifs

wip on eq_reas

fix for ci

simplify respectul and run proof

Doors do preserve safe !

Add respectful_run_inv v1

make hoare an explicit monad

airlock to eq_reas : :white_check_mark:

wip

examples/airlock.v
@@ -4,12 +4,14 @@
 
 (* Copyright (C) 2018–2020 ANSSI *)
 
-From Coq Require Import Arith.
 From FreerDPS Require Import Init.
-From FreerDPS Require Import Core Freer Hoare.
+(* WARNING: Move this import to its MathComp counterpart. *)
+From Stdlib Require Import Arith.
+From mathcomp Require Import all_boot classical_sets.
+From FreerDPS Require Import Core Freer Hoare HoareFacts.
+From examples Require Import airlock_helper.
 
-#[local] Open Scope nat_scope.
-#[local] Open Scope monae_scope.
+Import SpecializedHoareModule.
 
 Create HintDb airlock.
 
@@ -19,8 +21,7 @@ Create HintDb airlock.
 
 Inductive door : Type := left | right.
 
-Definition door_eq_dec (d d' : door) : { d = d' } + { ~ d = d' } :=
-  ltac:(decide equality).
+HB.instance Definition _ := gen_eqMixin door.
 
 Inductive DOORS : effect :=
 | IsOpen : door -> DOORS bool
@@ -28,24 +29,22 @@ Inductive DOORS : effect :=
 
 Generalizable All Variables.
 
-Arguments request {_ } _ _ _.
+Section airlock_s.
 
-Check request.
+Import FreerFuns.
 
-Section a.
-
-Definition is_open `{Provide Fx DOORS} {im : freerMonad Fx}
-    (d : door) : im bool :=
+Definition is_open `{Provide Fx DOORS} {im : freerMonad Fx} (d : door) :
+    im bool :=
   trigger (inj_p $ IsOpen d).
 
-Definition toggle `{Provide Fx DOORS} {im : freerMonad Fx}
-    (d : door) : im unit :=
+Definition toggle `{Provide Fx DOORS} {im : freerMonad Fx} (d : door) :
+    im unit :=
   trigger (inj_p $ Toggle d).
 
 Definition open_door `{Provide Fx DOORS} {im : freerMonad Fx}
     (d : door) : im unit :=
   is_open d >>= fun open =>
-  when (negb open) (toggle d).
+  when (~~ open) (toggle d).
 
 Definition close_door `{Provide Fx DOORS} {im : freerMonad Fx}
     (d : door) : im unit :=
@@ -71,11 +70,13 @@ Definition co (d : door) : door :=
   | right => left
   end.
 
+Lemma co_leftE : co left = right.
+Proof. by []. Qed.
+
 Definition controller `{Provide Fx DOORS, Provide Fx (STORE nat)}
-    {im : freerMonad Fx}
-  : component (im:=im) CONTROLLER Fx
+    {im : freerMonad Fx} : component (im:=im) CONTROLLER Fx
   (* .
-  move=>X; case=>[|d].
+  move=> X; case=> [|d].
   - apply/bind=>[|cpt].
     + apply/iget.
     + apply/when.
@@ -96,14 +97,14 @@ Definition controller `{Provide Fx DOORS, Provide Fx (STORE nat)}
     match op with
     | Tick =>
       iget >>= fun cpt =>
-      when (15 <? cpt) $
+      when (15 <? cpt)%nat $
         close_door left >>
         close_door right >>
-        iput 0
+        iput 0%nat
     | RequestOpen d =>
-        close_door (co d) >>
-        open_door d >>
-        iput 0
+      close_door (co d) >>
+      open_door d >>
+      iput 0%nat
     end.
 
 (** * Verifying the Airlock Controller *)
@@ -113,6 +114,7 @@ Definition controller `{Provide Fx DOORS, Provide Fx (STORE nat)}
 (** *** Witness States *)
 
 Definition Ω : Type := bool * bool.
+(*         S : Type := left * rght. *)
 
 Definition sel (d : door) : Ω -> bool :=
   match d with
@@ -122,23 +124,17 @@ Definition sel (d : door) : Ω -> bool :=
 
 Definition tog (d : door) (ω : Ω) : Ω :=
   match d with
-  | left => (negb (fst ω), snd ω)
-  | right => (fst ω, negb (snd ω))
+  | left => (~~ (fst ω), snd ω)
+  | right => (fst ω, ~~ (snd ω))
   end.
 
 Lemma tog_equ_1 (d : door) (ω : Ω)
-  : sel d (tog d ω) = negb (sel d ω).
-
-Proof.
-  by case:d.
-Qed.
+  : sel d (tog d ω) = ~~ (sel d ω).
+Proof. by case: d. Qed.
 
 Lemma tog_equ_2 (d : door) (ω : Ω)
   : sel (co d) (tog d ω) = sel (co d) ω.
-
-Proof.
-  destruct d; reflexivity.
-Qed.
+Proof. by case: d. Qed.
 
 (** From now on, we will reason about [tog] using [tog_equ_1] and [tog_equ_2].
     FreeSpec tactics rely heavily on [cbn] to simplify certain terms, so we use
@@ -150,130 +146,208 @@ Qed.
     theorems. *)
 
 #[local] Opaque tog.
+Opaque denote.
 
-Definition step (ω : Ω) (a : Type) (e : DOORS a) (x : a) :=
-  match e with
-  | Toggle d => tog d ω
-  | _ => ω
-  end.
+(* Ω = bool * bool : doors state *)
+Definition step (ω : Ω) (a : Type) (op : DOORS a) (_ : a) : Ω :=
+  if op is Toggle d then tog d ω else ω.
 
-(** *** Requirements *)
-
+(** *** Requirements / Precondition *)
 Inductive doors_o_caller : Ω -> forall (a : Type), DOORS a -> Prop :=
-
 (** - Given the door [d] of o system [ω], it is always possible to ask for the
       state of [d]. *)
-
 | req_is_open (d : door) (ω : Ω)
   : doors_o_caller ω bool (IsOpen d)
-
 (** - Given the door [d] of o system [ω], if [d] is closed, then the second door
       [co d] has to be closed too for a request to toggle [d] to be valid. *)
-
-| req_toggle (d : door) (ω : Ω) (H : sel d ω = false -> sel (co d) ω = false)
+| req_toggle (d : door) (ω : Ω) (H : sel (co d) ω -> sel d ω)
   : doors_o_caller ω unit (Toggle d).
+  (* H : ~~ sel (co d) ω *)
 
-Hint Constructors doors_o_caller : airlock.
-
-(** *** Promises *)
-
+(** *** Promises / PostCondition *)
 Inductive doors_o_callee : Ω -> forall (a : Type), DOORS a -> a -> Prop :=
-
 (** - When a system in a state [ω] reports the state of the door [d], it shall
       reflect the true state of [d]. *)
-
 | doors_o_callee_is_open (d : door) (ω : Ω) (x : bool) (equ : sel d ω = x)
   : doors_o_callee ω bool (IsOpen d) x
-
-(** - There is no particular doors_o_calleeises on the result [x] of a request for [ω] to
-      close the door [d]. *)
-
+(** - There is no particular requirement on the result [x] of a request for
+      [ω] to close the door [d]. *)
 | doors_o_callee_toggle (d : door) (ω : Ω) (x : unit)
   : doors_o_callee ω unit (Toggle d) x.
 
- Hint Constructors doors_o_callee : airlock.
-
 Definition doors_contract : contract DOORS Ω :=
   make_contract step doors_o_caller doors_o_callee.
+(* => {{door_caller}} p%step {{door_callee}} *)
+
+Lemma doors_effect_preE {Fx a} `{MayProvide Fx DOORS}
+    (op : Fx a) (ω : Ω) :
+  pre (hoare_of_contract doors_contract op) ω <->
+  match proj_p op with
+  | Some door_op => doors_o_caller ω a door_op
+  | None => True
+  end.
+Proof. by rewrite /hoare_of_contract /= /gen_caller_obligation. Qed.
+
+Lemma doors_o_caller_preE `{Provide Fx DOORS} {a}
+    (ω : Ω) (op : DOORS a) :
+  pre (hoare_of_contract doors_contract (inj_p op)) ω <->
+  doors_o_caller ω a op.
+Proof. by rewrite doors_effect_preE proj_inj_p_equ. Qed.
+
+Lemma doors_o_caller_preI `{Provide Fx DOORS} {a}
+    (ω : Ω) (op : DOORS a) :
+  doors_o_caller ω a op ->
+  pre (hoare_of_contract doors_contract (inj_p op)) ω.
+Proof. by rewrite doors_o_caller_preE. Qed.
+
+Lemma doors_effect_postE {Fx a} `{MayProvide Fx DOORS}
+    (op : Fx a) (ω : Ω) (x : a) (ω' : Ω) :
+  post (hoare_of_contract doors_contract op) ω x ω' <->
+  match proj_p op with
+  | Some door_op =>
+      ω' = step ω a door_op x /\ doors_o_callee ω a door_op x
+  | None => ω' = ω
+  end.
+Proof.
+rewrite /hoare_of_contract /= /gen_witness_update
+  /gen_callee_obligation.
+case: (proj_p op)=> [door_op |] /=.
+- by [].
+by split=> [[-> _] | ->].
+Qed.
+
+Lemma doors_o_callee_postE `{Provide Fx DOORS} {a}
+    (ω : Ω) (op : DOORS a) (x : a) (ω' : Ω) :
+  post (hoare_of_contract doors_contract (inj_p op)) ω x ω' <->
+  ω' = step ω a op x /\ doors_o_callee ω a op x.
+Proof. by rewrite doors_effect_postE proj_inj_p_equ. Qed.
+
+Lemma doors_other_effect_postE {Fx a} `{MayProvide Fx DOORS}
+    (op : Fx a) (other : proj_p op = None)
+    (ω : Ω) (x : a) (ω' : Ω) :
+  post (hoare_of_contract doors_contract op) ω x ω' <-> ω' = ω.
+Proof.
+by rewrite doors_effect_postE other.
+Qed.
+
+Opaque hoare_of_contract.
 
 (** ** Intermediary Lemmas *)
+Lemma doors_is_open_calleeE (ω : Ω) (d : door) (x : bool) :
+  doors_o_callee ω bool (IsOpen d) x -> sel d ω = x.
+Proof. by case: x=> postc; inversion postc; ssubst. Qed.
+
+Lemma doors_is_open_effect_retE `{Provide Fx DOORS}
+    (ω : Ω) (d : door) (opened : bool) (ω' : Ω) :
+  post (hoare_of_contract doors_contract
+          (A := bool) (inj_p (IsOpen d))) ω opened ω' <->
+  post (@ret (hoare Ω) bool (sel d ω)) ω opened ω'.
+Proof.
+rewrite doors_o_callee_postE hoare_pure_postE /=.
+split=> [ [-> callee] | [<- <-] ]; split=> //.
+- exact: doors_is_open_calleeE callee.
+- exact: doors_o_callee_is_open.
+Qed.
+
+Lemma doors_is_open_effect_ret_callerE `{Provide Fx DOORS}
+    (ω : Ω) (d : door) :
+  pre (hoare_of_contract doors_contract
+          (A := bool) (inj_p (IsOpen d))) ω <->
+  pre (@ret (hoare Ω) bool (sel d ω)) ω.
+Proof.
+by rewrite hoare_pure_preE; split=> // _;
+  apply: doors_o_caller_preI; exact: req_is_open.
+Qed.
+
+Lemma doors_toggle_effect_postE `{Provide Fx DOORS}
+  (ω : Ω) (d : door) (u : unit) (ω' : Ω) :
+  post (hoare_of_contract doors_contract
+          (A := unit) (inj_p (Toggle d))) ω u ω' <->
+  ω' = tog d ω.
+Proof.
+by rewrite doors_o_callee_postE;
+  split=> [ [-> _] | ->] //; split=>//;
+  exact: doors_o_callee_toggle.
+Qed.
+
+Lemma doors_toggle_effect_ret_callerE `{Provide Fx DOORS}
+    (ω : Ω) (d : door)
+    (* Safe : porte 1 ferméE -> porte 2 ferméE *)
+    (* (safe : sel d ω = false -> sel (co d) ω = false) *)
+    (safe : sel (co d) ω -> sel d ω) :
+  pre (hoare_of_contract doors_contract
+          (A := unit) (inj_p (Toggle d))) ω <->
+  pre (@ret (hoare Ω) unit tt) ω.
+Proof.
+by rewrite hoare_pure_preE; split=> // _;
+  apply: doors_o_caller_preI; exact: req_toggle safe.
+Qed.
+
+
+Lemma doors_toggle_callerE (ω : Ω) (d : door) :
+  doors_o_caller ω unit (Toggle d) ->
+  sel (co d) ω -> sel d ω.
+Proof. by move: ω d=> [[|] [|]] [|] //=; inversion 1. Qed.
 
 (** Closing a door [d] in any system [ω] is always a respectful operation. *)
+Local Open Scope classical_set_scope.
 
+
+(* TODO(cleanup): Check whether this proof can be shortened. *)
 Lemma close_door_respectful `{Provide Fx DOORS} {im : freerMonad Fx}
-    (ω : Ω) (d : door)
-  : pre (to_hoare
-      (im:=freer Fx)
-      doors_contract (close_door d)) ω.
-
+    (d : door) :
+  pre (to_hoare (im:=im) doors_contract (close_door d)) = [set: _].
 Proof.
-  prove impure with airlock; subst ; constructor.
-
-  (* This leaves us with one goal to prove:
-
-       [sel d ω = false -> sel (co d) ω = false]
-
-     Yet, thanks to our call to [IsOpen d], we can predict that
-
-       [sel d ω = true] *)
-
-  inversion o_caller0; ssubst.
-  now rewrite H3.
+rewrite /close_door -subTset=> ω _; apply: to_hoare_bind_preI.
+- by rewrite to_hoare_requestE doors_is_open_effect_ret_callerE.
+move=> [|] ω';
+  rewrite to_hoare_when_preE // to_hoare_requestE doors_is_open_effect_retE
+  => -[d_open <-].
+by rewrite to_hoare_requestE;
+  apply/(doors_toggle_effect_ret_callerE ω d).
 Qed.
 
- Hint Resolve close_door_respectful : airlock.
-
-Lemma open_door_respectful `{Provide Fx DOORS} (ω : Ω)
-    (d : door) (safe : sel (co d) ω = false)
-  : pre (to_hoare
-      (im:=freer Fx)
-      doors_contract (open_door (Fx:=Fx) d)) ω.
-
+(* TODO(cleanup): Check whether this proof can be shortened. *)
+Lemma open_door_respectful `{Provide Fx DOORS} {im : freerMonad Fx}
+    (ω : Ω) (d : door) (safe : ~~ sel (co d) ω) :
+  pre (to_hoare (im:=im) doors_contract
+    (open_door (Fx := Fx) d)) ω.
 Proof.
-  prove impure; repeat constructor; subst.
-  by inversion o_caller0; ssubst.
+rewrite /open_door; apply: to_hoare_bind_preI.
+- by rewrite to_hoare_requestE doors_is_open_effect_ret_callerE.
+move=> [|] ω'; rewrite to_hoare_when_preE //
+  to_hoare_requestE doors_is_open_effect_retE
+  => -[_ <-].
+rewrite to_hoare_requestE;
+  apply/(doors_toggle_effect_ret_callerE ω d)=>//.
+by move: safe=> /[swap] ->.
 Qed.
 
- Hint Resolve open_door_respectful : airlock.
-
-Lemma close_door_run `{Provide Fx DOORS} (ω : Ω) (d : door) (ω' : Ω) (x : unit)
-  (run : post
-    (to_hoare (im:=freer Fx)
-      doors_contract (close_door d)) ω x ω')
-  : sel d ω' = false.
+Lemma close_door_run `{Provide Fx DOORS} {im : freerMonad Fx}
+  (ω : Ω) (d : door) (ω' : Ω) (x : unit)
+  (run : post (to_hoare (im:=im) doors_contract (close_door d)) ω x ω') :
+~~ sel d ω'.
 Proof.
-  run_simpl run;
-  cleanvert H1.
-  cleanvert run.
-  cleanvert H1.
-  run_simpl H2.
-
-  cleanvert H2.
-  (* cleanvert H4. *)
-
-  -  cleanvert H1.
-    by rewrite tog_equ_1 H5.
-  by  cleanvert run.
+move: run; rewrite /close_door to_hoare_bind_postE.
+move=> [opened [? [ ]]].
+rewrite to_hoare_requestE doors_is_open_effect_retE to_hoare_when_postE
+  => -[+ <-].
+case: opened.
+- by move=> + [[] ];
+  rewrite to_hoare_requestE doors_toggle_effect_postE=> /[swap] ->;
+  rewrite tog_equ_1=> ->.
+by move=> /[swap] -> ->.
 Qed.
-
- Hint Resolve close_door_run : airlock.
 
 #[local] Opaque close_door.
 #[local] Opaque open_door.
 #[local] Opaque Nat.ltb.
 
 Remark one_door_safe_all_doors_safe (ω : Ω) (d : door)
-    (safe : sel d ω = false \/ sel (co d) ω = false)
-  : forall (d' : door), sel d' ω = false \/ sel (co d') ω = false.
-
+    (safe : ~~sel d ω \/ ~~sel (co d) ω)
+  : forall (d' : door), ~~sel d' ω \/ ~~sel (co d') ω.
 Proof.
-  intros d'.
-  destruct d; destruct d'; auto.
-  + cbn -[sel].
-    now rewrite or_comm.
-  + cbn -[sel].
-    fold (co right).
-    now rewrite or_comm.
+by move: d safe=> + /[swap]; case; case=>//=; rewrite or_comm.
 Qed.
 
 (** The objective of this lemma is to prove that, if either the right door or
@@ -281,19 +355,60 @@ Qed.
     [p] that interacts with doors, this fact remains true. *)
 
 #[local] Opaque sel.
+Definition doors_safe (ω : Ω) :=
+  ~~ sel left ω \/ ~~ sel right ω.
+
+(* TODO(cleanup): Check whether this proof can be shortened. *)
+Lemma doors_request_preserves_safe `{Provide Fx DOORS}
+    {im : freerMonad Fx}
+    `(op : Fx a) (ω : Ω) (x : a) (ω' : Ω) :
+  pre (to_hoare (im:=im) doors_contract (trigger op)) ω ->
+  post (to_hoare (im:=im) doors_contract (trigger op)) ω x ω' ->
+  doors_safe ω -> doors_safe ω'.
+Proof.
+rewrite to_hoare_requestE doors_effect_preE doors_effect_postE.
+case: (proj_p op)=> [door_op |] /=; last first.
+- by move=> _ ->.
+move=> + [-> _].
+move: door_op x; case=> d [] caller safe //=.
+apply: (one_door_safe_all_doors_safe _ d).
+move: safe=> /one_door_safe_all_doors_safe /(_ d).
+case=> [d_closed | ?]; right; rewrite tog_equ_2 //.
+apply/negP=> co_open; move/negP: d_closed=> d_closed.
+by inversion caller as [|?? Hsafe]; subst;
+  move: co_open Hsafe d_closed=> -> ->.
+Qed.
+
+Lemma doors_handler_preserves_safe `{Provide Fx DOORS}
+    {im : freerMonad Fx} {A} (op : Fx A) :
+  preserves_invariant doors_safe
+    (hoare_of_contract doors_contract op).
+Proof.
+by move=> state result state' op_pre op_post state_safe;
+  apply: (doors_request_preserves_safe (im:=im) op state result state');
+  rewrite ?to_hoare_requestE.
+Qed.
+
+Lemma doors_run_preserves_safe `{Provide Fx DOORS}
+    {A} (p : freer Fx A) :
+  preserves_invariant doors_safe
+    (p |= doors_contract).
+Proof.
+elim: p=> [value | X op k IH].
+- by rewrite to_hoare_localE; exact: preserves_invariant_ret.
+exact: (preserves_invariant_bind
+  (doors_handler_preserves_safe (im:=freer Fx) op) IH).
+Qed.
 
 Lemma respectful_run_inv `{Provide Fx DOORS} {A} (p : freer Fx A)
-    (ω : Ω) (safe : sel left ω = false \/ sel right ω = false)
+    (ω : Ω) (safe : ~~ sel left ω \/ ~~ sel right ω)
     (a : A) (ω' : Ω)
-    (hpre : pre
-      (to_hoare (im:=freer Fx)
-        doors_contract p) ω)
-    (hpost : post
-      (to_hoare (im:=freer Fx)
-        doors_contract p) ω a ω')
-  : sel left ω' = false \/ sel right ω' = false.
-
-(** We reason by induction on the impure computation [p]:
+    (hpre : pre (to_hoare (im:=freer Fx) doors_contract p) ω)
+    (hpost : post (to_hoare (im:=freer Fx) doors_contract p) ω a ω') :
+  ~~ sel left ω' \/ ~~ sel right ω'.
+(** The induction in [doors_run_preserves_safe] reduces this proof to showing
+    that every handled request preserves [doors_safe]. It accounts for the
+    following two cases:
 
     - Either [p] is a pure computation; in such a case, the doors state
       does not change, hence the proof is trivial.
@@ -322,67 +437,46 @@ Lemma respectful_run_inv `{Provide Fx DOORS} {A} (p : freer Fx A)
          closed after the request has been handled.  Because there is at least
          one door closed ([co d]), we can conclude that either the right or the
          left door is closed thanks to [one_door_safe_all_doors_safe]. *)
-
 Proof.
-  fold (co left) in *.
-  revert ω hpre hpost safe.
-  (* elim p=>[a'|B e f IH] ω pre run safe. *)
-  induction p; intros ω hpre run safe.
-  + by unroll_post run.
-  + run_simpl run.
-    have hpost : post (hoare_of_contract doors_contract (A:=β) op) ω x ω0
-      by split; [apply H2| by rewrite H3].
-    (* move: H1 => /(_ x ω0) => H1. *)
-     apply/(H1 x ω0) => //; [by apply hpre|].
-    cbn in *.
-    inversion hpre; rewrite /=/gen_caller_obligation in H4.
-    (* simplify_gens *)
-    unfold gen_caller_obligation, gen_callee_obligation, gen_witness_update in *.
-    cbn in *.
-    destruct (proj_p op) as [e'|].
-    ++ destruct hpost as [o_callee equω].
-       destruct e' as [d|d].
-       +++ rewrite H3.
-           apply safe.
-       +++ apply one_door_safe_all_doors_safe with (d := d);
-             apply one_door_safe_all_doors_safe with (d' := d) in safe;
-             subst.
-             inversion H4.
-           cbn.
-           by destruct safe as [safe|safe];
-            right; rewrite tog_equ_2//.
-    ++ rewrite H3;
-       exact: safe.
+by move: hpre hpost safe; exact: doors_run_preserves_safe.
 Qed.
 
-Lemma controller_correct `{StrictProvide2 Fx DOORS (STORE nat)}
-  : correct_component
-      (im:=freer Fx) controller
-                      (no_contract CONTROLLER)
-                      doors_contract
-                      (fun _ ω => sel left ω = false \/ sel right ω = false).
+(** ** Main Theorem *)
+(* TODO(cleanup): Check whether this proof can be shortened. *)
+Theorem controller_correct
+    `{StrictProvide2 Fx DOORS (STORE nat)}
+  : correct_component controller
+    (im:=freer Fx)
+    (no_contract CONTROLLER)
+    doors_contract
+    (fun _ ω => ~~ sel left ω \/ ~~ sel right ω).
 Proof.
-  move=>ωc ωd pred A eff req.
-  have hpre : pre
-      (to_hoare (im:=freer Fx)
-        doors_contract (controller A eff)) ωd.
-    {
-      case eff; do ! [prove impure with airlock; ssubst; constructor => //].
-
-
-      (* case eff=> [|d]//; prove impure with airlock; ssubst; constructor=>//. *)
-        (* do ! [prove impure with airlock; ssubst; constructor=>//=].  *)
-      - by inversion o_caller; ssubst; rewrite H6.
-      - by inversion o_caller1; ssubst; rewrite H6.
-      - by inversion o_caller0; ssubst; rewrite H6.
-      - by inversion o_caller; ssubst; rewrite H6.
-      - by inversion o_caller1; ssubst;inversion o_caller; ssubst; rewrite H6 tog_equ_1/=H7.
-      - by inversion o_caller; ssubst.
-    }
-
-  split=>[|a ωE' run]//=;
-  split=>//=.
-  by apply/(respectful_run_inv _ _ _ _ _ _ run).
+rewrite /correct_component=> ωF ω safe α op _.
+have controller_pre :
+    pre (to_hoare doors_contract
+      (controller (im:=freer Fx) α op)) ω.
+  case: op=> [|d]; rewrite /controller.
+  - apply: to_hoare_bind_preI.
+    + exact: to_hoare_distinguished_request_preI.
+    move=> cpt state /to_hoare_distinguished_request_postE ->.
+    rewrite to_hoare_when_preE.
+    case: (15 <? cpt)%nat=> //=.
+    apply: to_hoare_bind_preI.
+    + by apply: to_hoare_bind_preI=>
+        [|result state' close_post]; rewrite close_door_respectful.
+    by move=> result state' closes_post;
+      exact: to_hoare_distinguished_request_preI.
+  apply: to_hoare_bind_preI.
+  - apply: to_hoare_bind_preI.
+    + by rewrite close_door_respectful.
+    move=> result state close_post.
+    exact: (open_door_respectful (Fx:=Fx) (im:=freer Fx) state d
+      (close_door_run ω (co d) state result close_post)).
+  by move=> result state body_post;
+    exact: to_hoare_distinguished_request_preI.
+split=> // x ω' run; split; first exact: mk_no_callee_obligation.
+exact: (respectful_run_inv (Fx:=Fx)
+  (controller (im:=freer Fx) α op) ω safe x ω' controller_pre run).
 Qed.
 
-End a.
+End airlock_s.
