theories/Contract.v
@@ -11,7 +11,6 @@
     semantics (according to a certain definition of “correct”). *)
 
 From FreerDPS Require Import Init.
-(* From ExtLib Require Import StateMonad MonadState MonadTrans. *)
 From FreerDPS Require Import Effect Freer.
 #[local]
 Open Scope signature_scope.
@@ -40,19 +39,19 @@ Generalizable All Variables.
     To keep this state up-to-date after each primitive interpretation,
     contracts also define a dedicated function [witness_update]. *)
 
-Record contract (F : effect) (Ω : Type) : Type := make_contract
-  { witness_update (ω : Ω) : forall (α : Type), F α -> α -> Ω
-  ; caller_obligation (ω : Ω) : forall (α : Type),  F α -> Prop
-  ; callee_obligation (ω : Ω) : forall (α : Type), F α -> α -> Prop
+Record contract (F : effect) (St : Type) : Type := make_contract
+  { witness_update (*state_upd*) : St -> forall (α : Type), F α -> α -> St
+  ; caller_obligation(*precond*) : St -> forall (α : Type), F α -> Prop
+  ; callee_obligation(*postcond*) : St -> forall (α : Type), F α -> α -> Prop
   }.
 
 Declare Scope contract_scope.
 Bind Scope contract_scope with contract.
 
-Arguments make_contract [F Ω] (_ _ _).
-Arguments witness_update [F Ω] (c ω) [α] (_ _).
-Arguments caller_obligation [F Ω] (c ω) [α] (_).
-Arguments callee_obligation [F Ω] (c ω) [α] (_ _).
+Arguments make_contract [F St] (_ _ _).
+Arguments witness_update [F St] (c s) [α] (_ _).
+Arguments caller_obligation [F St] (c s) [α] (_).
+Arguments callee_obligation [F St] (c s) [α] (_ _).
 
 (** The most simple contract we can define is the one that requires
     anything both for the impure computations which uses the primitives of a
@@ -60,15 +59,16 @@ Arguments callee_obligation [F Ω] (c ω) [α] (_ _).
     these primitives. *)
 
 Definition const_witness {F} :=
-  fun (u : unit) (α : Type) (e : F α) (x : α) => u.
+  fun (u : unit) (α : Type) (op : F α) (x : α) => u.
 
-Inductive no_caller_obligation {F Ω} (ω : Ω) (α : Type) (e : F α) : Prop :=
-| mk_no_caller_obligation : no_caller_obligation ω α e.
+Inductive no_caller_obligation {F St} (s : St) (α : Type) (op : F α) : Prop :=
+| mk_no_caller_obligation : no_caller_obligation s α op.
 
 #[global] Hint Constructors no_caller_obligation : freespec.
 
-Inductive no_callee_obligation {F Ω} (ω : Ω) (α : Type) (e : F α) (x : α) : Prop :=
-| mk_no_callee_obligation : no_callee_obligation ω α e x.
+Inductive no_callee_obligation {F St} (s : St) (α : Type)
+    (op : F α) (x : α) : Prop :=
+| mk_no_callee_obligation : no_callee_obligation s α op x.
 
 #[global] Hint Constructors no_callee_obligation : freespec.
 
@@ -81,7 +81,7 @@ Definition no_contract (F : effect) : contract F unit :=
 (** A similar —and as simple— contract is the one that forbids the use of a
     given effect. *)
 
-Definition do_no_use {F Ω} (ω : Ω) (α : Type) (e : F α) : Prop := False.
+Definition do_no_use {F St} (s : St) (α : Type) (op : F α) : Prop := False.
 
 Definition forbid_specs (F : effect) : contract F unit :=
   {| witness_update := const_witness
@@ -91,61 +91,61 @@ Definition forbid_specs (F : effect) : contract F unit :=
 
 (** * Contract Equivalence *)
 
-Definition contract_caller_equ `(c1 : contract F Ω1) `(c2 : contract F Ω2)
-    (f : Ω1 -> Ω2)
+Definition contract_caller_equ `(c1 : contract F S1) `(c2 : contract F S2)
+    (f : S1 -> S2)
   : Prop :=
-  forall ω1 a (p : F a),
-    caller_obligation c1 ω1 p <-> caller_obligation c2 (f ω1) p.
+  forall s1 a (p : F a),
+    caller_obligation c1 s1 p <-> caller_obligation c2 (f s1) p.
 
-Definition contract_callee_equ `(c1 : contract F Ω1) `(c2 : contract F Ω2)
-    (f : Ω1 -> Ω2)
+Definition contract_callee_equ `(c1 : contract F S1) `(c2 : contract F S2)
+    (f : S1 -> S2)
   : Prop :=
-  forall ω1 a (p : F a) x,
-    callee_obligation c1 ω1 p x <-> callee_obligation c2 (f ω1) p x.
+  forall s1 a (p : F a) x,
+    callee_obligation c1 s1 p x <-> callee_obligation c2 (f s1) p x.
 
-Definition contract_witness_equ `(c1 : contract F Ω1) `(c2 : contract F Ω2)
-    (f : Ω1 -> Ω2)
+Definition contract_witness_equ `(c1 : contract F S1) `(c2 : contract F S2)
+    (f : S1 -> S2)
   : Prop :=
-  forall ω1 a (p : F a) x,
-    f (witness_update c1 ω1 p x) = witness_update c2 (f ω1) p x.
+  forall s1 a (p : F a) x,
+    f (witness_update c1 s1 p x) = witness_update c2 (f s1) p x.
 
-Inductive contract_equ `(c1 : contract F Ω1) `(c2 : contract F Ω2)
+Inductive contract_equ `(c1 : contract F S1) `(c2 : contract F S2)
   : Type :=
-| mk_contract_equ (f : Ω1 -> Ω2) (g : Ω2 -> Ω1)
+| mk_contract_equ (f : S1 -> S2) (g : S2 -> S1)
     (iso1 : forall x, f (g x) = x) (iso2 : forall x, g (f x) = x)
     (caller_equ : contract_caller_equ c1 c2 f)
     (callee_equ : contract_callee_equ c1 c2 f)
     (witness_equ : contract_witness_equ c1 c2 f)
   : contract_equ c1 c2.
 
-Definition contract_iso_lr `(c1 : contract F Ω1) `(c2 : contract F Ω2)
-    (equ : contract_equ c1 c2) (ω1 : Ω1)
-  : Ω2 :=
+Definition contract_iso_lr `(c1 : contract F S1) `(c2 : contract F S2)
+    (equ : contract_equ c1 c2) (s1 : S1)
+  : S2 :=
   match equ with
-  | @mk_contract_equ _ _ _ _ _ f _ _ _ _ _ _ => f ω1
+  | @mk_contract_equ _ _ _ _ _ f _ _ _ _ _ _ => f s1
   end.
 
-Definition contract_iso_rl `(c1 : contract F Ω1) `(c2 : contract F Ω2)
-    (equ : contract_equ c1 c2) (ω2 : Ω2)
-  : Ω1 :=
+Definition contract_iso_rl `(c1 : contract F S1) `(c2 : contract F S2)
+    (equ : contract_equ c1 c2) (s2 : S2)
+  : S1 :=
   match equ with
-  | @mk_contract_equ _ _ _ _ _ _ g _ _ _ _ _ => g ω2
+  | @mk_contract_equ _ _ _ _ _ _ g _ _ _ _ _ => g s2
   end.
 
-Arguments contract_iso_lr {F Ω1 c1 Ω2 c2} (equ ω1).
-Arguments contract_iso_rl {F Ω1 c1 Ω2 c2} (equ ω2).
+Arguments contract_iso_lr {F S1 c1 S2 c2} (equ s1).
+Arguments contract_iso_rl {F S1 c1 S2 c2} (equ s2).
 
-Lemma contract_equ_refl `(c : contract F Ω)
+Lemma contract_equ_refl `(c : contract F St)
   : contract_equ c c.
 
 Proof.
   apply mk_contract_equ with (f:=fun x => x) (g:=fun x => x); auto.
-  + now intros ω α p.
-  + now intros ω α p x.
-  + now intros ω α p x.
+  + now intros s α p.
+  + now intros s α p x.
+  + now intros s α p x.
 Defined.
 
-Lemma contract_equ_sym `(c1 : contract F Ω1) `(c2 : contract F Ω2)
+Lemma contract_equ_sym `(c1 : contract F S1) `(c2 : contract F S2)
    (equ : contract_equ c1 c2)
   : contract_equ c2 c1.
 
@@ -154,26 +154,26 @@ Proof.
   apply mk_contract_equ with (f:=g) (g:=f).
   + apply iso2.
   + apply iso1.
-  + intros ω α p.
-    transitivity (caller_obligation c2 (f (g ω)) p).
+  + intros s α p.
+    transitivity (caller_obligation c2 (f (g s)) p).
     ++ now rewrite iso1.
     ++ now symmetry.
-  + intros ω α p x.
-    transitivity (callee_obligation c2 (f (g ω)) p x).
+  + intros s α p x.
+    transitivity (callee_obligation c2 (f (g s)) p x).
     ++ now rewrite iso1.
     ++ now symmetry.
-  + intros ω α p x.
-    rewrite <- (iso2 (witness_update c1 (g ω) p x)).
-    assert (equ : witness_update c2 ω p x = f (witness_update c1 (g ω) p x)). {
-      transitivity (witness_update c2 (f (g ω)) p x).
+  + intros s α p x.
+    rewrite <- (iso2 (witness_update c1 (g s) p x)).
+    assert (equ : witness_update c2 s p x = f (witness_update c1 (g s) p x)). {
+      transitivity (witness_update c2 (f (g s)) p x).
       + now rewrite iso1.
       + now rewrite witness_equ.
     }
     now rewrite equ.
 Defined.
 
-Lemma contract_equ_trans `(c1 : contract F Ω1) `(c2 : contract F Ω2)
-   `(c3 : contract F Ω3)
+Lemma contract_equ_trans `(c1 : contract F S1) `(c2 : contract F S2)
+   `(c3 : contract F S3)
    `(is_equ12 : contract_equ c1 c2)
    `(is_equ23 : contract_equ c2 c3)
   : contract_equ c1 c3.
@@ -187,16 +187,16 @@ Proof.
     now setoid_rewrite isofg23.
   + setoid_rewrite isogf23.
     now setoid_rewrite isogf12.
-  + intros ω1 α p.
-    transitivity (caller_obligation c2 (f12 ω1) p);
+  + intros s1 α p.
+    transitivity (caller_obligation c2 (f12 s1) p);
       [ now apply caller_equ12
       | now apply caller_equ23 ].
-  + intros ω1 α p x.
-    transitivity (callee_obligation c2 (f12 ω1) p x); [ now apply callee_equ12
+  + intros s1 α p x.
+    transitivity (callee_obligation c2 (f12 s1) p x); [ now apply callee_equ12
                                                       | now apply callee_equ23 ].
-  + intros ω1 α p x.
+  + intros s1 α p x.
     rewrite <- witness_equ23.
-    assert (equ : f12 (witness_update c1 ω1 p x) = witness_update c2 (f12 ω1) p x)
+    assert (equ : f12 (witness_update c1 s1 p x) = witness_update c2 (f12 s1) p x)
       by now rewrite <- witness_equ12.
     now rewrite equ.
 Defined.
@@ -204,45 +204,54 @@ Defined.
 (** * Composing Contracts *)
 
 (** As we compose effects and operational semantics, we can easily compose
-    contracts together, by means of the [contractprod] operator. Given [F] and [E]
-    two effects, if we can reason about [F] and [E] independently (e.g., the
-    caller obligations of [E] do not vary when we use [F]), then we can compose
-    [ci : contract F ΩF] and [cj : contract E ΩE], such that [contractprod ci cj] in a
-    contract for [F + E]. *)
+    contracts together, by means of the [contractprod] operator. Given [F]
+    and [E], two effects, if we can reason about [F] and [E] independently
+    (e.g., the caller obligations of [E] do not vary when we use [F]), then we
+    can compose [cF : contract F SF] and [cE : contract E SE], such that
+    [contractprod cF cE] is a contract for [F + E]. *)
 
-Definition gen_witness_update `{MayProvide Fx F} {Ω α} (c : contract F Ω)
-    (ω :  Ω) (e : Fx α) (x : α)
-  : Ω :=
-  match proj_p e with
-  | Some e => witness_update c ω e x
-  | None => ω
+Definition gen_witness_update {Fx : effect} `{MayProvide Fx F} {St α}
+    (c : contract F St)
+    (s :  St) (op : Fx α) (x : α)
+  : St :=
+  match proj_p op with
+  | Some op => witness_update c s op x
+  | None => s
   end.
 
-Definition gen_caller_obligation `{MayProvide Fx F} {Ω α} (c : contract F Ω)
-    (ω :  Ω) (e : Fx α)
+Definition gen_caller_obligation {Fx : effect} `{MayProvide Fx F} {St α}
+    (c : contract F St)
+    (s :  St) (op : Fx α)
   : Prop :=
-  match proj_p e with
-  | Some e => caller_obligation c ω e
+  match proj_p op with
+  | Some op => caller_obligation c s op
   | None => True
   end.
 
-Definition gen_callee_obligation `{MayProvide Fx F} {Ω α} (c : contract F Ω)
-    (ω :  Ω) (e : Fx α) (x : α)
+Definition gen_callee_obligation {Fx : effect} `{MayProvide Fx F} {St α}
+    (c : contract F St)
+    (s :  St) (op : Fx α) (x : α)
   : Prop :=
-  match proj_p e with
-  | Some e => callee_obligation c ω e x
+  match proj_p op with
+  | Some op => callee_obligation c s op x
   | None => True
   end.
 
-Definition contractprod `{Provide Fx F, Provide Fx E} {ΩF ΩE}
-    (ci : contract F ΩF) (cj : contract E ΩE)
-  : contract Fx (ΩF * ΩE) :=
-  {| witness_update := fun (ω : ΩF * ΩE) (α : Type) (e : Fx α) (x : α) =>
-                         (gen_witness_update ci (fst ω) e x, gen_witness_update cj (snd ω) e x)
-  ;  caller_obligation := fun (ω : ΩF * ΩE) (α : Type) (e : Fx α) =>
-                       gen_caller_obligation ci (fst ω) e /\ gen_caller_obligation cj (snd ω) e
-  ;  callee_obligation := fun (ω : ΩF * ΩE) (α : Type) (e : Fx α) (x : α) =>
-                   gen_callee_obligation ci (fst ω) e x /\ gen_callee_obligation cj (snd ω) e x
+Definition contractprod {Fx : effect} `{Provide Fx F, Provide Fx E} {SF SE}
+    (cF : contract F SF) (cE : contract E SE)
+  : contract Fx (SF * SE) :=
+  {| witness_update :=
+       fun (s : SF * SE) (α : Type) (op : Fx α) (x : α) =>
+         (gen_witness_update cF (fst s) op x,
+          gen_witness_update cE (snd s) op x)
+  ; caller_obligation :=
+      fun (s : SF * SE) (α : Type) (op : Fx α) =>
+        gen_caller_obligation cF (fst s) op /\
+        gen_caller_obligation cE (snd s) op
+  ; callee_obligation :=
+      fun (s : SF * SE) (α : Type) (op : Fx α) (x : α) =>
+        gen_callee_obligation cF (fst s) op x /\
+        gen_callee_obligation cE (snd s) op x
   |}.
 
 Infix "*" := contractprod : contract_scope.
@@ -252,27 +261,27 @@ Infix "*" := contractprod : contract_scope.
 
 (* FIXME: Should be [StrictProvide2 Fx F E] *)
 
-Definition sharedcontractprod `{Provide Fx F, Provide Fx E}
-   `(ci : contract F Ω) (cj : contract E Ω)
-  : contract Fx Ω :=
+Definition sharedcontractprod {Fx : effect} `{Provide Fx F, Provide Fx E}
+   `(cF : contract F St) (cE : contract E St)
+  : contract Fx St :=
   {|
   witness_update :=
-    fun (ω : Ω) (α : Type) (e : Fx α) (x : α) =>
+    fun (s : St) (α : Type) (op : Fx α) (x : α) =>
       (* we need to check [F] before [E] because [sharedcontractprod]
          will be right associative *)
-      match proj_p (F:=F) e with
-      | Some e => witness_update ci ω e x
-      | _ => match proj_p (F:=E) e with
-             | Some e => witness_update cj ω e x
-             | _ => ω
+      match proj_p (F:=F) op with
+      | Some op => witness_update cF s op x
+      | _ => match proj_p (F:=E) op with
+             | Some op => witness_update cE s op x
+             | _ => s
              end
       end;
   caller_obligation :=
-    fun (ω : Ω) (α : Type) (e : Fx α) =>
-      gen_caller_obligation ci ω e /\ gen_caller_obligation cj ω e;
+    fun (s : St) (α : Type) (op : Fx α) =>
+      gen_caller_obligation cF s op /\ gen_caller_obligation cE s op;
   callee_obligation :=
-    fun (ω : Ω) (α : Type) (e : Fx α) (x : α) =>
-      gen_callee_obligation ci ω e x /\ gen_callee_obligation cj ω e x
+    fun (s : St) (α : Type) (op : Fx α) (x : α) =>
+      gen_callee_obligation cF s op x /\ gen_callee_obligation cE s op x
   |}.
 
 Infix "^" := sharedcontractprod  : contract_scope.
@@ -294,8 +303,8 @@ Inductive STORE (s : Type) : effect :=
     s) s], and the witness will be updated after each [Put] call. *)
 
 Definition store_update (s : Type) :=
-  fun (x : s) (α : Type) (e : STORE s α) (_ : α) =>
-    match e with
+  fun (x : s) (α : Type) (op : STORE s α) (_ : α) =>
+    match op with
     | Get => x
     | Put x' => x'
     end.
