theories/Hoare.v
@@ -39,11 +39,14 @@ Arguments post {Σ α} (_ _ _).
 Definition hoare_pure {Σ α} (x : α) : hoare Σ α :=
   mk_hoare [set: Σ] (fun s y s' => x = y /\ s = s').
 
-Definition hoare_bind {Σ α β} (h : hoare Σ α) (k : α -> hoare Σ β) : hoare Σ β :=
+Definition hoare_bind {Σ α β}
+    (h : hoare Σ α) (k : α -> hoare Σ β) : hoare Σ β :=
   mk_hoare (fun s => pre h s /\ (forall x s', post h s x s' -> pre (k x) s'))
            (fun s x s'' => exists y s', post h s y s' /\ post (k y) s' x s'').
 
 (** * Instances *)
+
+
 
 (** ** Functor *)
 
@@ -57,6 +60,15 @@ Definition hoare_apply {Σ α β} (hf : hoare Σ (α -> β)) (h : hoare Σ α)
   hoare_bind hf (fun f => hoare_map f h).
 
 (** ** Monad *)
+
+(** A nominal class for monads with Hoare semantics. *)
+HB.mixin Record isMonadHoare (S : UU0)
+    (M : UU0 -> UU0) of Monad M := {}.
+
+#[short(type=hoareMonad)]
+HB.structure Definition MonadHoare (S : UU0) :=
+  {M of isMonadHoare S M &}.
+
 Module hoare_mon.
 Section hm.
 Variable Σ : UU0.
@@ -120,17 +132,97 @@ End hoare_mon.
 
 HB.export hoare_mon.
 
+HB.instance Definition _ (S : UU0) :=
+  isMonadHoare.Build S (hoare S).
+
+(** ** Primitive Views *)
+
+Lemma hoare_pureE {Σ α} (x : α) :
+  @ret (hoare Σ) α x = @hoare_pure Σ α x.
+Proof. by []. Qed.
+
+Lemma hoare_bindE {Σ α β} (h : hoare Σ α) (k : α -> hoare Σ β) :
+  @bind (hoare Σ) α β h k = hoare_bind h k.
+Proof. by []. Qed.
+
+Lemma hoare_pure_preE {Σ α} (x : α) s :
+  pre (@ret (hoare Σ) α x) s <-> True.
+Proof. by rewrite hoare_pureE /hoare_pure. Qed.
+
+Lemma hoare_pure_postE {Σ α} (x y : α) s s' :
+  post (@ret (hoare Σ) α x) s y s' <-> x = y /\ s = s'.
+Proof. by rewrite hoare_pureE /hoare_pure. Qed.
+
+Lemma hoare_bind_preE {Σ α β} (h : hoare Σ α) (k : α -> hoare Σ β) s :
+  pre (h >>= k) s <->
+  pre h s /\ (forall x s', post h s x s' -> pre (k x) s').
+Proof. by rewrite hoare_bindE /hoare_bind. Qed.
+
+Lemma hoare_bind_postE {Σ α β} (h : hoare Σ α)
+    (k : α -> hoare Σ β) s x s'' :
+  post (h >>= k) s x s'' <->
+  exists y s', post h s y s' /\ post (k y) s' x s''.
+Proof. by rewrite hoare_bindE /hoare_bind. Qed.
+
+Lemma hoare_ext {Σ α} (h1 h2 : hoare Σ α) :
+  (forall s, pre h1 s <-> pre h2 s) ->
+  (forall s x s', post h1 s x s' <-> post h2 s x s') ->
+  h1 = h2.
+Proof.
+  case: h1 => pre1 post1; case: h2 => pre2 post2.
+  move=> pre_equiv post_equiv /=.
+  congr mk_hoare.
+  - apply/boolp.funext=> s.
+    exact/boolp.propext/pre_equiv.
+  apply/eq3_fun=> s x s'.
+  exact/boolp.propext/post_equiv.
+Qed.
+
+(** ** Invariant Preservation *)
+
+Definition preserves_invariant {S A}
+    (invariant : S -> Prop) (h : hoare S A) :=
+  forall state result state',
+    pre h state ->
+    post h state result state' ->
+    invariant state ->
+    invariant state'.
+
+Lemma preserves_invariant_ret {S A}
+    (invariant : S -> Prop) (result : A) :
+  preserves_invariant invariant (@ret (hoare S) A result).
+Proof.
+by move=> state result' state' _ /hoare_pure_postE [_ <-].
+Qed.
+
+Lemma preserves_invariant_bind {S A B} (invariant : S -> Prop)
+    (h : hoare S A) (k : A -> hoare S B) :
+  preserves_invariant invariant h ->
+  (forall result, preserves_invariant invariant (k result)) ->
+  preserves_invariant invariant (h >>= k).
+Proof.
+by move=> h_preserves k_preserves state result state'
+  /hoare_bind_preE [h_pre k_pre]
+  /hoare_bind_postE [x [statex [h_post k_post]]] state_safe;
+exact: k_preserves x statex result state'
+  (k_pre x statex h_post) k_post
+  (h_preserves state x statex h_pre h_post state_safe).
+Qed.
+
 (** * Reasoning about Programs *)
 
-Definition hoare_of_contract `{MayProvide Fx F} `(c : contract F Ω)
+Definition hoare_of_contract {Fx : effect} `{MayProvide Fx F}
+    `(c : contract F Ω)
     : Fx ~~> hoare Ω :=
-  fun a e => mk_hoare
-    (fun ω => gen_caller_obligation c ω e)
-    (fun ω x ω' => gen_callee_obligation c ω e x /\
-                   ω' = gen_witness_update c ω e x).
+  fun a op => mk_hoare
+    (gen_caller_obligation c ^~ op)
+    (fun ω x ω' => ω' = gen_witness_update c ω op x /\
+                  gen_callee_obligation c ω op x).
 
 Definition to_hoare `{MayProvide Fx F} {im : freerMonad Fx}
     `(c : contract F Ω)
     : im ~~> hoare Ω :=
   denote _ (hoare_of_contract c).
 Arguments to_hoare {Fx F _ im Ω} c {α} : rename.
+
+Notation "p |= c" := (to_hoare c p) (at level 70).
