theories/Component.v
@@ -87,6 +87,8 @@ Definition bootstrap {F} {im : freerMonad eempty}
     of type [c : compoment E Fx s]. *)
 Local Open Scope monae_scope.
 
+Section tmp.
+Import Freer.
 
 #[local]
 Fixpoint with_component_aux {Fx E α}
@@ -99,14 +101,11 @@ Fixpoint with_component_aux {Fx E α}
   : freer Fx α :=
   match p with
   | pure x => pure x
-  | impure T (in_right e) f =>
-    c T e >>= fun res => with_component_aux c (f res)
-  | impure _ (in_left e) f =>
-    impure e (fun x => with_component_aux c (f x))
+  | impure T (in_right op) k =>
+    c T op >>= fun res => with_component_aux c (k res)
+  | impure _ (in_left op) k =>
+    impure op (fun x => with_component_aux c (k x))
   end.
-
-Notation "m >>= f" := (freer_bind m f).
-Notation "m >> f" := (freer_bind m (fun _ => f)).
 
 Definition with_component {Fx E α}
   (* `{im : freerMonad Fx}
@@ -122,3 +121,5 @@ Definition with_component {Fx E α}
   with_component_aux c p >>= fun res =>
   finalizer >>
   pure res.
+
+End tmp.
