theories/HoareFacts.v
@@ -10,175 +10,272 @@ Attributes deprecated(
 From FreerDPS Require Import Init Effect Freer Contract Hoare.
 Generalizable All Variables.
 
-(** * General Lemmas *)
+Local Open Scope monae_scope.
 
-Lemma to_hoare_step `{MayProvide Fx F} `(c : contract F Ω)
-   `(e : Fx a) `(f : a -> freer Fx a)
-   `(hpre : pre
-      (to_hoare (im:=freer Fx) c (impure e f)) ω)
-    (x : a) (step : gen_callee_obligation c ω e x)
-  : pre
-      (to_hoare (im:=freer Fx) c (f x))
-      (gen_witness_update c ω e x).
+(** * Hoare Interpretation Views *)
 
+Section GenericHoareSection.
+Variable Fx : effect.
+Context `{MayProvide Fx F} {im : freerMonad Fx} `(c : contract F Ω).
+
+(* Lemma hoare_of_contract_preE `(op : Fx a) (ω : Ω) :
+  pre (hoare_of_contract c op) ω <-> gen_caller_obligation c ω op.
+Proof. by split. Qed.
+
+Lemma hoare_of_contract_postE `(op : Fx a) (ω : Ω) (x : a) (ω' : Ω) :
+  post (hoare_of_contract c op) ω x ω' <->
+  ω' = gen_witness_update c ω op x /\
+  gen_callee_obligation c ω op x.
+Proof. by split. Qed.
+
+Lemma hoare_of_contract_postI `(op : Fx a) (ω : Ω) (x : a) :
+  gen_callee_obligation c ω op x ->
+  post (hoare_of_contract c op) ω x (gen_witness_update c ω op x).
+Proof. by move=> step; split. Qed. *)
+
+Lemma to_hoare_requestE `(op : Fx a) :
+  to_hoare (im:=im) c (request a op) = hoare_of_contract c op.
+Proof. exact: denote_request. Qed.
+
+(* Lemma to_hoare_request_preE `(op : Fx a) (ω : Ω) :
+  pre (to_hoare (im:=im) c (request a op)) ω <->
+  gen_caller_obligation c ω op.
+Proof. by rewrite to_hoare_requestE hoare_of_contract_preE. Qed.
+
+Lemma to_hoare_request_postE `(op : Fx a) (ω : Ω) (x : a) (ω' : Ω) :
+  post (to_hoare (im:=im) c (request a op)) ω x ω' <->
+  ω' = gen_witness_update c ω op x /\ gen_callee_obligation c ω op x.
+Proof. by rewrite to_hoare_requestE hoare_of_contract_postE. Qed.
+
+Lemma to_hoare_request_postI `(op : Fx a) (ω : Ω) (x : a) :
+  gen_callee_obligation c ω op x ->
+  post (to_hoare (im:=im) c (request a op)) ω x
+       (gen_witness_update c ω op x).
+Proof. by rewrite to_hoare_requestE; exact: hoare_of_contract_postI. Qed. *)
+
+(* ============ *)
+Context `(p : im a) `(f : a -> im b).
+
+Lemma to_hoare_bindE :
+  to_hoare c (p >>= f) =
+  to_hoare c p >>= fun x => to_hoare c (f x).
+Proof. exact: denote_bind. Qed.
+
+Lemma to_hoare_bind_preE (ω : Ω) :
+  pre (to_hoare c (p >>= f)) ω <->
+  pre (to_hoare c p) ω /\
+  forall x ω',
+    post (to_hoare c p) ω x ω' -> pre (to_hoare c (f x)) ω'.
+Proof. by rewrite to_hoare_bindE hoare_bind_preE. Qed.
+
+Lemma to_hoare_bind_preI (ω : Ω) :
+  pre (to_hoare c p) ω ->
+  (forall x ω',
+    post (to_hoare c p) ω x ω' ->
+    pre (to_hoare c (f x)) ω') ->
+  pre (to_hoare c (p >>= f)) ω.
+Proof. by move=> prefix suffix; apply/to_hoare_bind_preE; split. Qed.
+
+Lemma to_hoare_bind_postE (ω : Ω) (y : b) (ω' : Ω) :
+  post (to_hoare c (p >>= f)) ω y ω' <->
+  exists x ω'',
+    post (to_hoare c p) ω x ω'' /\ post (to_hoare c (f x)) ω'' y ω'.
+Proof. by rewrite to_hoare_bindE hoare_bind_postE. Qed.
+
+Lemma to_hoare_bind_postI
+    (ω : Ω) (x : a) (ω'' : Ω) (y : b) (ω' : Ω) :
+  post (to_hoare c p) ω x ω'' ->
+  post (to_hoare c (f x)) ω'' y ω' ->
+  post (to_hoare c (p >>= f)) ω y ω'.
 Proof.
-  destruct hpre as [hbefore hafter].
-  apply hafter.
-  cbn.
-  unfold gen_callee_obligation, gen_witness_update in *.
-  now destruct proj_p.
+by move=> prefix suffix; apply/to_hoare_bind_postE; exists x, ω''.
 Qed.
 
-#[global] Hint Resolve to_hoare_step : freespec.
-
-Lemma to_hoare_pre_bind_assoc `{MayProvide Fx F} `(c : contract F Ω)
-   `(p : freer Fx a)
-   `(Hp : pre
-      (to_hoare (im:=freer Fx) c p) ω)
-   `(f : a -> freer Fx b)
+Lemma to_hoare_pre_bind_assoc
+    `(Hp : pre (to_hoare c p) ω)
     (run : forall (x : a) (ω' : Ω),
-      post
-        (to_hoare (im:=freer Fx) c p)
-        ω x ω' ->
-      pre
-        (to_hoare (im:=freer Fx) c (f x)) ω')
-  : pre
-      (to_hoare (im:=freer Fx) c (freer_bind p f)) ω.
+      post (to_hoare c p) ω x ω' ->
+      pre (to_hoare c (f x)) ω') :
+  pre (to_hoare c (p >>= f)) ω.
+Proof. exact/to_hoare_bind_preI. Qed.
 
+Lemma to_hoare_post_bind_assoc
+    `(Hp : post (to_hoare c (p >>= f)) ω x ω') :
+  exists y ω'',
+    post (to_hoare c p) ω y ω'' /\
+    post (to_hoare c (f y)) ω'' x ω'.
+Proof. exact/to_hoare_bind_postE. Qed.
+
+End GenericHoareSection.
+
+Module SpecializedHoareModule.
+Section SpecializedHoareSection.
+Variable Fx : effect.
+Context `{MayProvide Fx F} `(c : contract F Ω).
+
+Lemma to_hoare_localE `(x : a) : (pure x |= c) = Ret x.
+Proof. exact: denote_ret. Qed.
+
+Lemma to_hoare_local_preE `(x : a) (ω : Ω) : pre (pure x |= c) ω.
+Proof. by rewrite to_hoare_localE hoare_pure_preE. Qed.
+
+Lemma to_hoare_local_preI `(x : a) (ω : Ω) : pre (pure x |= c) ω.
+Proof. by apply/to_hoare_local_preE. Qed.
+
+(* Lemma to_hoare_skip_preI (ω : Ω) :
+  pre (to_hoare c (skip : freer Fx unit)) ω.
+Proof. exact: to_hoare_local_preI. Qed. *)
+
+Lemma to_hoare_local_postE `(x : a) (y : a) (ω ω' : Ω) :
+  post (pure x |= c) ω y ω' <-> x = y /\ ω = ω'.
+Proof. by rewrite to_hoare_localE hoare_pure_postE. Qed.
+
+Lemma to_hoare_local_postI `(x : a) (ω : Ω) :
+  post (pure x |= c) ω x ω.
+Proof. by apply/to_hoare_local_postE; split. Qed.
+
+(* ========================================================================= *)
+Context `(op : Fx a) `(f : a -> freer Fx b).
+
+(* Lemma to_hoare_impure_preE (ω : Ω) :
+  pre (to_hoare c (impure op f)) ω <->
+  gen_caller_obligation c ω op /\ forall x, gen_callee_obligation c ω op x ->
+    pre (to_hoare c (f x)) (gen_witness_update c ω op x).
 Proof.
-  revert ω Hp run.
-  induction p; intros ω Hp run.
-  + now apply run.
-  + cbn in Hp.
-    destruct Hp as [He Hn].
-    split.
-    ++ exact He.
-    ++ intros x ω' Hpost.
-       specialize Hn with x ω'.
-       destruct Hpost.
-       rewrite -> H2 in *.
-       assert (Hpre : pre
-          (to_hoare (im:=freer Fx) c (f0 x))
-          (gen_witness_update c ω op x))
-         by now apply Hn.
-       apply H0; [ apply Hpre |].
-       intros y ω'' Hpost.
-       apply run.
-       cbn.
-       exists x.
-       exists ω'.
-       split; [split |].
-       +++ exact H1.
-       +++ exact H2.
-       +++ rewrite H2.
-           exact Hpost.
+split.
+- move=> /hoare_bind_preE [caller next]; split.
+  + exact/hoare_of_contract_preE.
+  + by move=> x callee; apply: next; exact/hoare_of_contract_postI.
+- move=> [caller next]; apply/hoare_bind_preE; split.
+  + exact/hoare_of_contract_preE.
+  + by move=> x ω' /hoare_of_contract_postE [-> callee]; exact: next.
 Qed.
 
-Lemma to_hoare_post_bind_assoc `{MayProvide Fx F} `(c : contract F Ω)
-   `(p : freer Fx a) `(f : a -> freer Fx b)
-   `(Hp : post
-      (to_hoare (im:=freer Fx) c (freer_bind p f)) ω x ω')
-  : exists y ω'',
-    post
-      (to_hoare (im:=freer Fx) c p) ω y ω'' /\
-    post
-      (to_hoare (im:=freer Fx) c $ f y) ω'' x ω'.
+Lemma to_hoare_impure_preI (ω : Ω) :
+  gen_caller_obligation c ω op ->
+  (forall x, gen_callee_obligation c ω op x ->
+    pre (to_hoare c (f x)) (gen_witness_update c ω op x)) ->
+  pre (to_hoare c (impure op f)) ω.
+Proof. by move=> caller next; apply/to_hoare_impure_preE; split. Qed.
 
+Lemma to_hoare_impure_postE (ω : Ω) (y : b) (ω' : Ω) :
+  post (to_hoare c (impure op f)) ω y ω' <->
+  exists x,
+    post (to_hoare c (f x)) (gen_witness_update c ω op x) y ω' /\
+    gen_callee_obligation c ω op x.
 Proof.
-move: ω Hp; elim p=>[in_a|Y op k IH] ω.
-- by exists in_a, ω.
-case=>y [ω'' [Hp1 ]].
-move:IH=>/[apply].
-move=> [z [ω''' [Hp2 Hp3]]].
-exists z, ω'''.
-split=>//.
-exists y, ω''.
-by split.
+split.
+- move=> /hoare_bind_postE [x [ω'' [+ suffix]]].
+  rewrite hoare_of_contract_postE.
+  by move=> [callee witness]; subst ω''; exists x.
+- move=> [x [callee suffix]]; apply/hoare_bind_postE.
+  by exists x, (gen_witness_update c ω op x); split.
 Qed.
 
-Lemma to_hoare_contractprod `{Provide Fx F, Provide Fx E}
-   `(ci : contract F ΩF) `(cj : contract E ΩE)
-   `(p : freer Fx a)
-   `(prei : pre
-      (to_hoare (im:=freer Fx) ci p) ωF)
-   `(prej : pre
-      (to_hoare (im:=freer Fx) cj p) ωE)
-  : pre
-      (to_hoare (im:=freer Fx) (ci * cj) p) (ωF, ωE).
+Lemma to_hoare_step `(hpre : pre (to_hoare c (impure op f)) ω)
+    (x : a) (step : gen_callee_obligation c ω op x) :
+  pre (to_hoare c (f x)) (gen_witness_update c ω op x).
+Proof. by move: hpre => /to_hoare_impure_preE [_ +]; exact. Qed. *)
 
+End SpecializedHoareSection.
+End SpecializedHoareModule.
+
+Import SpecializedHoareModule.
+
+
+(** * Contract Product Views *)
+
+(* Lemma contractprod_callerE {Fx : effect} `{Provide Fx F, Provide Fx E}
+    `(cF : contract F ΩF) `(cE : contract E ΩE)
+    (ωF : ΩF) (ωE : ΩE) `(op : Fx a) :
+  gen_caller_obligation (cF * cE) (ωF, ωE) op <->
+  gen_caller_obligation cF ωF op /\ gen_caller_obligation cE ωE op.
+Proof. by split. Qed.
+
+Lemma contractprod_calleeE {Fx : effect} `{Provide Fx F, Provide Fx E}
+    `(cF : contract F ΩF) `(cE : contract E ΩE)
+    (ωF : ΩF) (ωE : ΩE) `(op : Fx a) (x : a) :
+  gen_callee_obligation (cF * cE) (ωF, ωE) op x <->
+  gen_callee_obligation cF ωF op x /\
+  gen_callee_obligation cE ωE op x.
+Proof. by split. Qed.
+
+Lemma contractprod_witnessE {Fx : effect} `{Provide Fx F, Provide Fx E}
+    `(cF : contract F ΩF) `(cE : contract E ΩE)
+    (ωF : ΩF) (ωE : ΩE) `(op : Fx a) (x : a) :
+  gen_witness_update (cF * cE) (ωF, ωE) op x =
+  (gen_witness_update cF ωF op x, gen_witness_update cE ωE op x).
+Proof. by []. Qed. *)
+
+(* Lemma to_hoare_contractprod_preI
+    {Fx : effect} `{Provide Fx F, Provide Fx E}
+    `(cF : contract F ΩF) `(cE : contract E ΩE)
+    `(p : freer Fx a) (ωF : ΩF) (ωE : ΩE) :
+  pre (to_hoare cF p) ωF ->
+  pre (to_hoare cE p) ωE ->
+  pre (to_hoare (cF * cE) p) (ωF, ωE).
 Proof.
-  revert ωF prei ωE prej.
-  induction p; intros ωF prei ωE prej.
-  + auto.
-  + destruct prei as [calleri Hcalleei].
-    destruct prej as [callerj Hcalleej].
-    split.
-    ++ now split.
-    ++ intros x [ωF' ωE'] [[calleei calleej] equωs].
-       cbn in equωs.
-       inversion equωs; subst.
-       apply H3.
-       +++ apply Hcalleei.
-           now split.
-       +++ apply Hcalleej.
-           now split.
+move: p ωF ωE.
+elim=> [x | b op f ih] ωF ωE.
+  by move=> _ _; apply/to_hoare_local_preE.
+rewrite 2!to_hoare_impure_preE.
+move=> [callerF nextF] [callerE nextE].
+apply/to_hoare_impure_preI.
+  by apply/contractprod_callerE; split.
+move=> x /contractprod_calleeE [calleeF calleeE].
+rewrite contractprod_witnessE.
+apply: ih.
+  exact: nextF calleeF.
+exact: nextE calleeE.
 Qed.
 
-#[global] Hint Resolve to_hoare_contractprod : freespec.
+Lemma to_hoare_contractprod {Fx : effect} `{Provide Fx F, Provide Fx E}
+    `(cF : contract F ΩF) `(cE : contract E ΩE)
+    `(p : freer Fx a) `(preF : pre (to_hoare cF p) ωF)
+    `(preE : pre (to_hoare cE p) ωE) :
+  pre (to_hoare (cF * cE) p) (ωF, ωE).
+Proof. exact: to_hoare_contractprod_preI preF preE. Qed.
+
+#[global] Hint Resolve to_hoare_contractprod_preI : freespec.
+*)
 
 Lemma contract_equ_pre `(c1 : contract F Ω1) `(c2 : contract F Ω2)
-   `(equ : contract_equ c1 c2) (ω1 : Ω1)
-   `(p : freer F A)
-  : pre
-      (to_hoare (im:=freer F) c1 p) ω1 <->
-    pre
-      (to_hoare (im:=freer F) c2 p) (contract_iso_lr equ ω1).
-
+    `(equ : contract_equ c1 c2) (ω1 : Ω1) `(p : freer F A) :
+  pre (to_hoare c1 p) ω1 <->
+  pre (to_hoare c2 p) (contract_iso_lr equ ω1).
 Proof.
-  elim: equ => f g iso1 iso2 caller_equ callee_equ witness_equ.
-  move: ω1.
-  elim: p=> [a | B e k IH] ω1. 
-  - by split.
-  rewrite /=/gen_caller_obligation/gen_callee_obligation/gen_witness_update/=.
-  rewrite (caller_equ ω1 B e).
-  setoid_rewrite (callee_equ ω1 B e).
-  split => [[ocaller onext] | [ocaller onext]];
-  split => // x ω1' [ocallee owitness].
-  - by rewrite owitness -witness_equ -IH; eauto.
-  rewrite IH; eauto.
-  rewrite owitness /= witness_equ; eauto.
+elim: equ => f g iso1 iso2 caller_equ callee_equ witness_equ.
+move: ω1.
+elim: p=> [a | B op k IH] ω1.
+- by split.
+rewrite /= /gen_caller_obligation /gen_callee_obligation
+  /gen_witness_update /=.
+rewrite (caller_equ ω1 B op).
+setoid_rewrite (callee_equ ω1 B op).
+split => [[ocaller onext] | [ocaller onext]];
+  split => // x ω1' [owitness ocallee].
+- by rewrite owitness -witness_equ -IH; eauto.
+rewrite IH; eauto.
+rewrite owitness /= witness_equ; eauto.
 Qed.
 
 #[global] Hint Resolve contract_equ_pre : freespec.
 
 Lemma contract_equ_post `(c1 : contract F Ω1) `(c2 : contract F Ω2)
-   `(equ : contract_equ c1 c2) (ω1 ω1' : Ω1)
-   `(p : freer F a) (x : a)
-    (post1 : post
-      (to_hoare (im:=freer F) c1 p) ω1 x ω1')
-  : post
-      (to_hoare (im:=freer F) c2 p)
-      (contract_iso_lr equ ω1) x (contract_iso_lr equ ω1').
-
+    `(equ : contract_equ c1 c2) (ω1 ω1' : Ω1)
+    `(p : freer F A) (x : A)
+    (post1 : post (to_hoare c1 p) ω1 x ω1') :
+  post (to_hoare c2 p) (contract_iso_lr equ ω1) x
+       (contract_iso_lr equ ω1').
 Proof.
-  induction equ.
-  cbn in *.
-  revert x ω1 ω1' post1.
-  induction p; intros y ω1 ω1' post1.
-  + destruct post1 as [xequ ω1equ].
-    cbn.
-    now subst.
-  + cbn in post1.
-    destruct post1 as [x [ω1'' [[ocallee owitness] post1]]].
-    eapply H in post1.
-    exists x.
-    exists (f ω1'').
-    split; auto.
-    cbn.
-    repeat split.
-    ++ eapply callee_equ; eauto.
-    ++ rewrite owitness.
-       apply witness_equ.
+elim: equ => [f g iso1 iso2 caller_equ callee_equ witness_equ].
+move: p x ω1 ω1' post1.
+elim=> [in_a | B op k ih].
+- by move=> a ω1 ω1' [<- <-].
+move=> a ω1 ω1' [b [ω1'' [[ow oc] +]]] /= => /ih post1.
+exists b, (f ω1''); split; [split|exact: post1].
+- by rewrite ow witness_equ.
+- exact/(callee_equ ω1 B op).
 Qed.
 
 #[global] Hint Resolve contract_equ_post : freespec.
