theories/Instrument.v
@@ -14,7 +14,6 @@ Generalizable All Variables.
 
 Notation instrument Ω F := (stateT Ω (StateMonad.acto (semantics F))).
 
-
 Definition modify {S} {M : stateMonad S} (f : S -> S) : M S := get >>=
   fun s => put (f s) >>=
   fun _ => Ret s.
@@ -23,11 +22,10 @@ Arguments liftS {_ _ _}.
 Arguments effect_to_state {_ _}.
 
 
-Program Definition effect_to_instrument
-    `{MayProvide Fx F} `(c : contract F Ω)
-  : Fx ~~> instrument Ω Fx :=
+Program Definition interface_to_instrument `{MayProvide ix i} `(c : contract i Ω)
+  : ix ~~> instrument Ω ix :=
   fun a e =>
-    (liftS (A:=a) $ effect_to_state e)
+    (liftS (A:=a) $ interface_to_state e)
     >>= fun x => modify (fun ω => gen_witness_update c ω e x)
     >>= fun _ => Ret x.
 
